Intersection.thy
@@ -1,0 +1,15 @@
+theory Intersection
+imports Main
+begin
+
+section \<open> An auxiliary fact about closure under intersection\<close>
+
+lemma ne_family_intersection:
+  fixes X::"'node::finite set set"
+  assumes ne:"X \<noteq> {}" and all_ne:"\<And> x . x \<in> X \<Longrightarrow> x \<noteq> {}"
+    and closed:"\<And> A B . A \<in> X \<Longrightarrow> B \<in> X \<Longrightarrow> A \<inter> B \<in> X"
+  shows "\<Inter>X\<in>X"  \<comment> \<open>We assume this fact and check that it is okay with Nitpick\<close>
+  sorry
+
+end
+
